WIP

MPL/ProofMode/Tactics/VCGen.lean
@@ -12,6 +12,8 @@ import MPL.WPMonadFunctor
 import MPL.WPMonadExceptOf
 
 import MPL.ProofMode.Tactics.Intro
+import MPL.ProofMode.Tactics.Cases
+import MPL.ProofMode.Tactics.Specialize
 import MPL.ProofMode.Tactics.WP
 import MPL.ProofMode.Tactics.Spec
 import MPL.Triple
@@ -27,89 +29,190 @@ initialize registerTraceClass `mpl.tactics.vcgen
 
 namespace VC
 
-inductive ProofTerm where
-| rfl
-| nonrfl (e : Expr)
+theorem Specs.ite_pre {m} (c : Prop) [Decidable c] (t : m α) (e : m α)
+    {ps} [WP m ps] {P : Assertion ps} {Q₁ Q₂ : PostCond α ps}
+    (ht : c → ⦃P⦄ t ⦃Q₁⦄) (he : ¬c → ⦃P⦄ e ⦃Q₂⦄) :
+    ⦃P⦄ if c then t else e ⦃if c then Q₁ else Q₂⦄ := by
+  split <;> apply_rules
+
+theorem Specs.ite_post {m} (c : Prop) [Decidable c] (t : m α) (e : m α)
+    {ps} [WP m ps] {P₁ P₂ : Assertion ps} {Q : PostCond α ps}
+    (ht : c → ⦃P₁⦄ t ⦃Q⦄) (he : ¬c → ⦃P₂⦄ e ⦃Q⦄) :
+    ⦃if c then P₁ else P₂⦄ if c then t else e ⦃Q⦄ := by
+  split <;> apply_rules
+
+theorem split_ite {α m ps} {P : Assertion ps} {Q : PostCond α ps} (c : Prop) [Decidable c] [WP m ps] (t : m α) (e : m α)
+    (ht : c → ⦃P⦄ t ⦃Q⦄) (he : ¬c → ⦃P⦄ e ⦃Q⦄) :
+    ⦃P⦄ if c then t else e ⦃Q⦄ := by
+  split <;> apply_rules
+
+theorem Specs.bind_pre [Monad m] [WPMonad m ps] {x : m α} {f : α → m β} {P : Assertion ps} {Q : PostCond β ps}
+    (h : ⦃P⦄ x ⦃(fun a => wp⟦f a⟧.apply Q, Q.2)⦄) :
+    ⦃P⦄ (x >>= f) ⦃Q⦄ := by
+  mintro _
+  mwp
+  exact h
 
 inductive Fuel where
 | limited (n : Nat)
 | unlimited
 deriving DecidableEq
 
-def Fuel.burnOne (fuel : Fuel) : Option Fuel :=
-  match fuel with
-  | Fuel.limited 0 => none
-  | Fuel.limited n => some (Fuel.limited (n - 1))
-  | Fuel.unlimited => Fuel.unlimited
+structure State where
+  fuel : Fuel := .unlimited
 
-partial def step (fuel : Fuel) (goal : MGoal) (subst : Array Expr) (discharge : MGoal → Array Expr → MetaM Expr) : MetaM (Fuel × Expr) := do
-  let some fuel := fuel.burnOne | return (fuel, ← discharge goal subst)
-  let T := goal.target.consumeMData
-  trace[mpl.tactics.vcgen] "target: {T}"
-  logInfo m!"target: {T}"
-  if let some _ := T.app3? ``SPred.imp then
-    return ← onImp
-  if T.isAppOf ``PredTrans.apply then
-    return ← onApply
-  return (fuel, ← discharge goal subst)
+abbrev VCGenM := StateRefT State MetaM
+
+def burnOne : VCGenM PUnit := do
+  let s ← get
+  match s.fuel with
+  | Fuel.limited 0 => return ()
+  | Fuel.limited (n + 1) => set { s with fuel := .limited n }
+  | Fuel.unlimited => return ()
+
+def ifOutOfFuel (x : VCGenM α) (k : VCGenM α) : VCGenM α := do
+  let s ← get
+  match s.fuel with
+  | Fuel.limited 0 => x
+  | _ => k
+
+structure Result where
+--  expr : Expr
+  proof? : Option Expr := none
+
+def isTrivial (e : Expr) : Bool := match e with
+  | .bvar .. => true
+  | .mvar .. => true
+  | .fvar .. => true
+  | .const .. => true
+  | .lit .. => true
+  | .sort .. => true
+  | .mdata _ e => isTrivial e
+  | .proj _ _ e => isTrivial e
+  | .lam .. => false
+  | .forallE .. => false
+  | .letE .. => false
+  | .app .. => false
+
+def withNonTrivialLetDecl (name : Name) (type : Expr) (val : Expr) (k : Expr → (Expr → VCGenM Expr) → VCGenM α) (kind : LocalDeclKind := .default) : VCGenM α :=
+  if isTrivial val then
+    k val pure
+  else
+    withLetDecl name type val (kind := kind) fun fv => do
+      k fv (liftM <| mkForallFVars #[fv] ·)
+
+partial def step (fuel : Fuel) (goal : MGoal) (subst : Array Expr) (discharge : Expr → Array Expr → VCGenM Expr) : MetaM Expr :=
+  StateRefT'.run' (onGoal goal subst) { fuel }
 where
-  onImp := do mIntro goal (← `(binderIdent| _)) (fun g => step fuel g subst discharge)
+  onFail (goal : MGoal) (subst : Array Expr) : VCGenM Expr := do
+    logInfo m!"onFail: {goal.toExpr}, subst: {subst}, substituted: {goal.toExpr.instantiate subst}"
+    return ← discharge goal.toExpr subst
 
-  onApply := do
+  -- TODO: Update
+  -- If `let { expr, proof? } := onGoal goal subst`,
+  -- then `expr` is defeq to `goal.toExpr` (modulo `subst`)
+  -- and `proof` is the proof of the goal.
+  -- TODO: Figure otu what to do with `none`
+  onGoal goal subst : VCGenM Expr := do
+    -- trace[mpl.tactics.vcgen] "target: {T}"
+    -- logInfo m!"target: {T}"
+    let f := goal.target.consumeMData.getAppFn
+    match f.constName? with
+    | some ``SPred.imp => onImp goal subst
+    | some ``PredTrans.apply => onApply goal subst
+    | _ => onFail goal subst
+
+  onImp goal subst : VCGenM Expr := ifOutOfFuel (onFail goal subst) do
+    burnOne
+    (·.2) <$> mIntro goal (← `(binderIdent| _)) (fun g =>
+        do return ((), ← onGoal g subst))
+
+  onApply goal subst : VCGenM Expr := ifOutOfFuel (onFail goal subst) do
     let args := goal.target.getAppArgs
-    let wp := args[2]!
+    let trans := args[2]!
     let Q := args[3]!
-    match_expr wp with
+    logInfo m!"apply: {trans}"
+    match_expr trans with
     | WP.wp m ps instWP α e =>
-      let us := wp.getAppFn.constLevels!
+      let us := trans.getAppFn.constLevels!
+      let u := us[0]!
       if let .letE x ty val body _nonDep := e then
-        return (fuel, ← withLetDecl x ty val fun fv => do
+        burnOne
+        return ← withNonTrivialLetDecl x ty val fun fv leave => do
         let subst := subst.push fv
         let wp' := mkApp5 (mkConst ``WP.wp us) m ps instWP α body
         let args' := args.set! 2 wp'
         let goal := { goal with target := mkAppN (mkConst ``PredTrans.apply) args' }
-        mkLetFVars #[fv] (← discharge goal subst))
-      logInfo m!"hyps: {(← getLocalHyps)}"
-      logInfo m!"e: {e}"
-      if e.isIte then
-        let ite_args := e.getAppArgs
-        -- TODO: Only do this if Q is not already a var
+        leave (← onApply goal subst)
+      let monad? ← OptionT.run do
+        let instMon ← OptionT.mk <| synthInstance? (mkApp (mkConst ``Monad [Level.zero, u])  m)
+        let instWPMon ← OptionT.mk <| synthInstance? (mkApp3 (mkConst ``WPMonad us) m ps instMon)
+        return (instMon, instWPMon)
+      match_expr e with
+      | ite α c instDec th el =>
+        burnOne
+        -- TODO: This duplicates Q. We should compute the strongest post for goal.hyps in the future.
+        let tprf ← withLocalDeclD `h c fun hc => do
+          -- let subst := subst.push hc -- hc does not occur in the term
+          let wpt := mkApp5 (mkConst ``WP.wp us) m ps instWP α th
+          let tprf ← onApply { goal with target := mkAppN (mkConst ``PredTrans.apply) (args.set! 2 wpt) } subst
+          mkLambdaFVars #[hc] tprf
+        let eprf ← withLocalDeclD `h (mkApp (mkConst ``Not) c) fun hnc => do
+          -- let subst := subst.push hnc -- hnc does not occur in the term
+          let wpe := mkApp5 (mkConst ``WP.wp us) m ps instWP α el
+          let eprf ← onApply { goal with target := mkAppN (mkConst ``PredTrans.apply) (args.set! 2 wpe) } subst
+          mkLambdaFVars #[hnc] eprf
+        let prf := mkApp5 (mkConst ``split_ite us) α m ps goal.hyps Q
+        let prf := mkApp5 prf c instDec instWP th el
+        let prf := mkApp2 prf tprf eprf
+        -- logInfo m!"prf: {prf}"
+        --check (prf.instantiateRev subst)
+        return prf
+      | Pure.pure _m _ _α a =>
+        burnOne
+        let some (instMon, instWPMon) := monad? | failure
+        return ← withNonTrivialLetDecl `a α a fun a leave => do
+        let subst := subst.push a -- TODO: Does the wrong thing when we don't bind a
+        let goal := { goal with target := mkAppN (mkApp (mkProj ``Prod 0 Q) a) args[4:] }
+        let prf₁ ← discharge goal.toExpr subst
+        let prf₂ := mkApp7 (mkConst ``Specs.pure) m ps instMon instWPMon α a Q
+        let prf ← mkAppM ``SPred.entails.trans #[prf₁, prf₂]
+        check prf
+        return ← leave prf
+      | Bind.bind _m _ α' _ x k =>
+        burnOne
+        let some (instMon, instWPMon) := monad? | failure
         let Qty := mkApp2 (mkConst ``PostCond) α ps
-        return (fuel, ← withLetDecl `Q Qty Q fun Q => do
-        let t := mkApp5 (mkConst ``WP.wp us) m ps instWP α (e.getArg! 3)
-        let e := mkApp5 (mkConst ``WP.wp us) m ps instWP α (e.getArg! 4)
-        let tapplyQ := mkAppN (mkConst ``PredTrans.apply) (args.set! 2 t |>.set! 3 Q)
-        let eapplyQ := mkAppN (mkConst ``PredTrans.apply) (args.set! 2 e |>.set! 3 Q)
-        let ret_ty := (← inferType tapplyQ)
-        let u ← getLevel ret_ty
-        let ite_args' := ite_args.set! 0 (← inferType tapplyQ) |>.set! 3 tapplyQ |>.set! 4 eapplyQ
-        let ite := mkAppN (mkConst ``ite [u]) ite_args'
-        let goal := { goal with target := ite }
-        mkLetFVars #[Q] (← discharge goal subst))
-      if e.isAppOf ``Pure.pure then
-        return (fuel, ← withLetDecl `a α (e.getArg! 3) fun a => do
-        let goal := { goal with target := mkAppN (mkApp (mkProj ``Prod 0 Q) a) args }
-        mkLetFVars #[a] (← discharge goal subst))
+        return ← withNonTrivialLetDecl `Q Qty Q fun Q leaveQ => do
+        let subst := subst.push Q
+        let name := match k with | .lam n .. => n | _ => `a
+        let kapplyQ ← withLocalDeclD name α' fun a => do
+          let wpk := mkApp5 (mkConst ``WP.wp us) m ps instWP α (k.betaRev #[a])
+          mkForallFVars #[a] (← onApply { goal with target := mkAppN (mkConst ``PredTrans.apply) (args.set! 2 wpk |>.set! 3 Q) } subst)
+        logInfo m!"kapplyQ: {kapplyQ}, type: {← inferType kapplyQ}"
+        let Q' ← mkAppM ``Prod.mk #[← inferType kapplyQ, mkProj ``Prod 1 Q]
+        logInfo m!"Q': {Q'}"
+        let wpx := mkApp5 (mkConst ``WP.wp us) m ps instWP α x
+        let prf ← onApply { goal with target := mkAppN (mkConst ``PredTrans.apply) (args.set! 2 wpx |>.set! 3 Q') } subst
+        let prf := mkApp (mkApp10 (mkConst ``Specs.bind_pre) m ps α' α instMon instWPMon x k goal.hyps Q) prf
+        leaveQ prf
+      | _ => return ← discharge goal.toExpr subst
       -- Split match-expressions
-      if let some info := isMatcherAppCore? (← getEnv) e then
-        let candidate ← id do
-          let args := e.getAppArgs
-          logInfo "e: {e}, args: {args}"
-          for i in [info.getFirstDiscrPos : info.getFirstDiscrPos + info.numDiscrs] do
-            if args[i]!.hasLooseBVars then
-              return false
-          return true
-        if candidate then
-          -- We could be even more deliberate here and use the `lifter` lemmas
-          -- for the match statements instead of the `split` tactic.
-          -- For now using `splitMatch` works fine.
-          -- return ← Split.splitMatch goal e
-          return (fuel, ← discharge goal subst)
-    | _ => return (fuel, ← discharge goal subst)
---    if wp.isAppOf ``WP.wp then
---      let_expr WP.wp m ps instWP α x := wp | throwError "target not a wp application {wp}"
---    match
-  return (fuel, ← discharge goal subst)
+      --if let some info := isMatcherAppCore? (← getEnv) e then
+      --  let candidate ← id do
+      --    let args := e.getAppArgs
+      --    logInfo "e: {e}, args: {args}"
+      --    for i in [info.getFirstDiscrPos : info.getFirstDiscrPos + info.numDiscrs] do
+      --      if args[i]!.hasLooseBVars then
+      --        return false
+      --    return true
+      --  if candidate then
+      --    -- We could be even more deliberate here and use the `lifter` lemmas
+      --    -- for the match statements instead of the `split` tactic.
+      --    -- For now using `splitMatch` works fine.
+      --    -- return ← Split.splitMatch goal e
+      --    return (fuel, ← discharge goal subst)
+    | _ => return ← discharge goal.toExpr subst
 
 end VC
 
@@ -118,8 +221,8 @@ elab "mvcgen_step" n:(num)? : tactic => do
   let (mvar, goal) ← mStart (← getMainGoal)
   mvar.withContext do
   let goals ← IO.mkRef []
-  mvar.assign (← Prod.snd <$> VC.step (fuel := .limited n) goal #[] fun hyp subst => do
-    let m ← mkFreshExprSyntheticOpaqueMVar (hyp.toExpr.instantiateRev subst)
+  mvar.assign (← VC.step (fuel := .limited n) goal #[] fun hyp subst => do
+    let m ← mkFreshExprSyntheticOpaqueMVar (hyp.instantiate subst)
     goals.modify (m.mvarId! :: ·)
     return m)
   replaceMainGoal (← goals.get)
@@ -128,8 +231,8 @@ elab "mvcgen" : tactic => do
   let (mvar, goal) ← mStart (← getMainGoal)
   mvar.withContext do
   let goals ← IO.mkRef []
-  mvar.assign (← Prod.snd <$> VC.step (fuel := .unlimited) goal #[] fun hyp subst => do
-    let m ← mkFreshExprSyntheticOpaqueMVar (hyp.toExpr.instantiateRev subst)
+  mvar.assign (← VC.step (fuel := .unlimited) goal #[] fun hyp subst => do
+    let m ← mkFreshExprSyntheticOpaqueMVar (hyp.instantiate subst)
     goals.modify (m.mvarId! :: ·)
     return m)
   replaceMainGoal (← goals.get)
@@ -149,6 +252,18 @@ abbrev fib_spec : Nat → Nat
 | 1 => 1
 | n+2 => fib_spec n + fib_spec (n+1)
 
+theorem fib_triple_vc : ⦃⌜True⌝⦄ fib_impl n ⦃⇓ r => r = fib_spec n⦄ := by
+  unfold fib_impl
+  mvcgen_step 5
+--  dsimp
+--  mintro _
+--  if h : n = 0 then simp [h] else
+--  simp only [h]
+--  mwp
+--  mspec Specs.forIn_list (⇓ (⟨a, b⟩, xs) => a = fib_spec xs.rpref.length ∧ b = fib_spec (xs.rpref.length + 1)) ?step
+--  case step => dsimp; intros; mintro _; mwp; simp_all
+--  simp_all [Nat.sub_one_add_one]
+
 theorem fib_triple : ⦃⌜True⌝⦄ fib_impl n ⦃⇓ r => r = fib_spec n⦄ := by
   unfold fib_impl
   dsimp
@@ -159,15 +274,3 @@ theorem fib_triple : ⦃⌜True⌝⦄ fib_impl n ⦃⇓ r => r = fib_spec n⦄ :
   mspec Specs.forIn_list (⇓ (⟨a, b⟩, xs) => a = fib_spec xs.rpref.length ∧ b = fib_spec (xs.rpref.length + 1)) ?step
   case step => dsimp; intros; mintro _; mwp; simp_all
   simp_all [Nat.sub_one_add_one]
-
-theorem fib_triple_vc : ⦃⌜True⌝⦄ fib_impl n ⦃⇓ r => r = fib_spec n⦄ := by
-  unfold fib_impl
-  mvcgen_step 3
---  dsimp
---  mintro _
---  if h : n = 0 then simp [h] else
---  simp only [h]
---  mwp
---  mspec Specs.forIn_list (⇓ (⟨a, b⟩, xs) => a = fib_spec xs.rpref.length ∧ b = fib_spec (xs.rpref.length + 1)) ?step
---  case step => dsimp; intros; mintro _; mwp; simp_all
---  simp_all [Nat.sub_one_add_one]
